examples/RTac/EvenOdd.v
@@ -1,0 +1,183 @@
+Require Import MirrorCore.Lambda.Expr.
+Require Import MirrorCore.Lambda.ExprUnify_simul.
+Require Import MirrorCore.RTac.RTac.
+Require McExamples.Simple.Simple.
+Require Import MirrorCore.syms.SymEnv.
+
+
+Inductive Even : nat -> Prop :=
+| E0 : Even 0
+| EO : forall n, Odd n -> Even (S n)
+with Odd : nat -> Prop :=
+| OE : forall n, Even n -> Odd (S n).
+
+Let typ := Simple.typ.
+Let func := SymEnv.func.
+Let tyNat := Simple.tyNat.
+Let tyProp := Simple.tyProp.
+Let tyArr := Simple.tyArr.
+
+Definition args : functions _ :=
+  from_list ({| ftype := tyNat ; fdenote := 0 |} ::
+             {| ftype := tyArr tyNat tyNat ; fdenote := S |} ::
+             {| ftype := tyArr tyNat tyProp ; fdenote := Even |} ::
+             {| ftype := tyArr tyNat tyProp ; fdenote := Odd |} :: nil).
+
+Let Zero_syn : expr typ func := ExprCore.Inj 1%positive.
+Let S_syn : expr typ func := ExprCore.Inj 2%positive.
+Let Even_syn : expr typ func := ExprCore.Inj 3%positive.
+Let Odd_syn : expr typ func := ExprCore.Inj 4%positive.
+
+Definition E0_syn : Lemma.lemma typ (expr typ func) (expr typ func) :=
+{| Lemma.vars := nil
+ ; Lemma.premises := nil
+ ; Lemma.concl := App Even_syn Zero_syn
+ |}.
+
+Definition EO_syn : Lemma.lemma typ (expr typ func) (expr typ func) :=
+{| Lemma.vars := tyNat :: nil
+ ; Lemma.premises := App Odd_syn (ExprCore.Var 0) :: nil
+ ; Lemma.concl := App Even_syn (App S_syn (ExprCore.Var 0))
+ |}.
+
+Definition OE_syn : Lemma.lemma typ (expr typ func) (expr typ func) :=
+{| Lemma.vars := tyNat :: nil
+ ; Lemma.premises := App Even_syn (ExprCore.Var 0) :: nil
+ ; Lemma.concl := App Odd_syn (App S_syn (ExprCore.Var 0))
+ |}.
+
+Local Existing Instance Simple.RType_typ.
+Local Instance RSym_func : RSym func := @RSym_func _ _ args.
+
+Local Instance Expr_expr : Expr _ (expr typ func) := @Expr_expr typ func _ _ _.
+Local Instance ExprOk_expr : @ExprOk _ _ (expr typ func) _ := @ExprOk_expr typ func _ _ _ _ _ _.
+(*
+Definition subst :=
+  FMapSubst.SUBST.raw (expr typ func).
+Local Instance Subst_subst : SubstI.Subst subst (expr typ func)
+  := FMapSubst.SUBST.Subst_subst _.
+Local Instance SubstUpdate_subst : SubstI.SubstUpdate subst (expr typ func)
+  := @FMapSubst.SUBST.SubstUpdate_subst _ _.
+*)
+
+Let APPLY_no_minify (l : Lemma.lemma typ (expr typ func) (expr typ func))
+: rtac typ (expr typ func) :=
+  (@APPLY typ (expr typ func) _ _ _ _
+          (fun subst _ _ => @exprUnify subst typ _ Simple.RType_typ _ _ _ _ 10) l).
+
+
+Let APPLY (l : Lemma.lemma typ (expr typ func) (expr typ func)) : rtac typ (expr typ func) :=
+  THEN (APPLY_no_minify l) (@MINIFY _ _ _ _ _).
+
+Theorem APPLY_sound : forall l,
+                        @Lemma.lemmaD _ _ _ _ _ (fun tus tvs e => exprD' tus tvs e tyProp) _ nil nil l ->
+                        rtac_sound (APPLY l).
+Proof. Admitted.
+
+Definition even_odd_tac : rtac typ (expr typ func) :=
+  REPEAT 2000 (FIRST (APPLY EO_syn ::
+                      APPLY OE_syn ::
+                      APPLY E0_syn :: nil)).
+
+Definition App' : expr typ func -> expr typ func -> expr typ func :=
+  @App _ _.
+
+Fixpoint build_n (n : nat) : expr typ func :=
+  match n with
+    | 0 => Zero_syn
+    | S n => App' S_syn (build_n n)
+  end.
+
+Definition runRTac_empty_goal (tac : rtac typ (expr typ func))
+           (goal : expr typ func)  :=
+  (@runOnGoals _ _ _ _ tac)
+        nil nil 0 0 _ (@TopSubst _ _ nil nil)
+        (@GGoal typ (expr typ func) goal).
+
+Theorem even_odd_tac_sound
+: rtac_sound even_odd_tac.
+  eapply REPEAT_sound.
+  eapply FIRST_sound.
+  constructor; [ eapply APPLY_sound; exact EO | ].
+  constructor; [ eapply APPLY_sound; exact OE | ].
+  constructor; [ eapply APPLY_sound; exact E0 | ].
+  constructor.
+Qed.
+
+
+(*Time Eval vm_compute in runRTac_empty_goal even_odd_tac (App Even_syn (build_n 1024)). *)
+
+Definition GoalD (us vs : env) (g : Goal typ (expr typ func)) : Prop :=
+  let (tus, us0) := split_env us in
+  let (tvs, vs0) := split_env vs in
+  match @goalD typ (expr typ func) _ _ _ tus tvs g with
+    | Some P => P us0 vs0
+    | None => False
+  end.
+
+Definition full_solved : @Result typ (expr typ func) (CTop nil nil) :=
+  Solved (TopSubst (expr typ func) nil nil).
+
+Theorem runGoal_sound
+: forall e,
+    runRTac_empty_goal even_odd_tac e = full_solved ->
+    GoalD nil nil (GGoal e).
+Proof.
+Admitted.
+
+(*
+Goal Even 1024.
+  Time repeat constructor.
+Time Qed.
+*)
+
+Require Import MirrorCore.Reify.Reify.
+
+Reify Declare Patterns patterns_simple := (expr typ func).
+Reify Declare Syntax reify_simple :=
+  { (@Patterns.CFirst _ ((@Patterns.CPatterns (expr typ func) patterns_simple) ::
+                         (@Patterns.CApp (expr typ func) (App')) :: nil))
+  }.
+
+Reify Pattern patterns_simple += (@RExact _ O) => (Zero_syn).
+Reify Pattern patterns_simple += (@RExact _ S) => (S_syn).
+Reify Pattern patterns_simple += (@RExact _ Even) => (Even_syn).
+Reify Pattern patterns_simple += (@RExact _ Odd) => (Odd_syn).
+
+Ltac solve_it trm :=
+  let k e :=
+    pose (eV := e) ;
+    (change (GoalD nil nil (GGoal eV))) ;
+    apply (@runGoal_sound eV) ; vm_compute; reflexivity
+  in
+  reify_expr reify_simple k [ True ] [ trm ].
+
+
+Ltac solve_it' trm :=
+  let k eV :=
+    (change (GoalD nil nil (GGoal eV))) ;
+    apply (@runGoal_sound eV) ; vm_compute; reflexivity
+  in
+  reify_expr bind reify_simple k [ True ] [ trm ].
+
+Ltac solve_it'' trm :=
+  let k e :=
+    pose (eV := e) ;
+    (change (GoalD nil nil (GGoal eV))) ;
+    apply (@runGoal_sound eV) ; vm_compute; reflexivity
+  in
+  reify_expr reify_simple k [ True ] [ trm ].
+
+Ltac solve_it''' trm :=
+  let k e :=
+    (change (GoalD nil nil (GGoal e))) ;
+    apply (@runGoal_sound e) ; vm_compute; reflexivity
+  in
+  reify_expr reify_simple k [ True ] [ trm ].
+
+Goal Even 1024.
+  Time  match goal with
+    | |- ?X =>
+      solve_it' X
+  end.
+Time Qed.
