examples/RTac/EvenOddConst.v
@@ -1,0 +1,211 @@
+Require Import MirrorCore.Lambda.Expr.
+Require Import MirrorCore.Lambda.ExprUnify_simul.
+Require Import MirrorCore.RTac.RTac.
+Require McExamples.Simple.Simple.
+Require Import MirrorCore.syms.SymEnv.
+Require Import MirrorCore.syms.SymSum.
+
+
+Inductive Even : nat -> Prop :=
+| E0 : Even 0
+| EO : forall n, Odd n -> Even (S n)
+with Odd : nat -> Prop :=
+| OE : forall n, Even n -> Odd (S n).
+
+Let typ := Simple.typ.
+Let func := (SymEnv.func + nat)%type.
+Let tyNat := Simple.tyNat.
+Let tyProp := Simple.tyProp.
+Let tyArr := Simple.tyArr.
+
+Definition args : functions _ :=
+  from_list ({| ftype := tyNat ; fdenote := 0 |} ::
+             {| ftype := tyArr tyNat tyNat ; fdenote := S |} ::
+             {| ftype := tyArr tyNat tyProp ; fdenote := Even |} ::
+             {| ftype := tyArr tyNat tyProp ; fdenote := Odd |} :: nil).
+
+Let Zero_syn : expr typ func := ExprCore.Inj (inl 1%positive).
+Let S_syn : expr typ func := ExprCore.Inj (inl 2%positive).
+Let Even_syn : expr typ func := ExprCore.Inj (inl 3%positive).
+Let Odd_syn : expr typ func := ExprCore.Inj (inl 4%positive).
+
+Definition E0_syn : Lemma.lemma typ (expr typ func) (expr typ func) :=
+{| Lemma.vars := nil
+ ; Lemma.premises := nil
+ ; Lemma.concl := App Even_syn Zero_syn
+ |}.
+
+Definition EO_syn : Lemma.lemma typ (expr typ func) (expr typ func) :=
+{| Lemma.vars := tyNat :: nil
+ ; Lemma.premises := App Odd_syn (ExprCore.Var 0) :: nil
+ ; Lemma.concl := App Even_syn (App S_syn (ExprCore.Var 0))
+ |}.
+
+Definition OE_syn : Lemma.lemma typ (expr typ func) (expr typ func) :=
+{| Lemma.vars := tyNat :: nil
+ ; Lemma.premises := App Even_syn (ExprCore.Var 0) :: nil
+ ; Lemma.concl := App Odd_syn (App S_syn (ExprCore.Var 0))
+ |}.
+
+Local Existing Instance Simple.RType_typ.
+Print RSym.
+Definition RSym_nat : @RSym typ _ nat :=
+{| typeof_sym := fun _ => Some tyNat
+ ; symD := fun x => x
+ ; sym_eqb := fun x y => Some (EqNat.beq_nat x y)
+ |}.
+
+
+Local Instance RSym_func : RSym func := RSym_sum (@RSym_func _ _ args) RSym_nat.
+Local Instance RSymOk_func : RSymOk RSym_func := @RSymOk_sum _ _ _ _ _ _ _ _.
+admit.
+Defined.
+
+Local Instance Expr_expr : Expr _ (expr typ func) := @Expr_expr typ func _ _ _.
+Local Instance ExprOk_expr : @ExprOk _ _ (expr typ func) _ := @ExprOk_expr typ func _ _ _ _ _ _.
+(*
+Definition subst :=
+  FMapSubst.SUBST.raw (expr typ func).
+Local Instance Subst_subst : SubstI.Subst subst (expr typ func)
+  := FMapSubst.SUBST.Subst_subst _.
+Local Instance SubstUpdate_subst : SubstI.SubstUpdate subst (expr typ func)
+  := @FMapSubst.SUBST.SubstUpdate_subst _ _.
+*)
+
+Let APPLY_no_minify (l : Lemma.lemma typ (expr typ func) (expr typ func)) : rtac typ (expr typ func) :=
+  (@APPLY typ (expr typ func) _ _ _ _
+          (fun subst _ _ => @exprUnify subst typ _ Simple.RType_typ _ _ _ _ 10) l).
+
+
+Let APPLY (l : Lemma.lemma typ (expr typ func) (expr typ func)) : rtac typ (expr typ func) :=
+  THEN (APPLY_no_minify l)
+       (@MINIFY _ _ _ _ _).
+
+Theorem APPLY_sound
+: forall l,
+    @Lemma.lemmaD _ _ _ _ _ (exprD'_typ0 (T:=Prop)) _ nil nil l ->
+    rtac_sound (APPLY l).
+Proof.
+  intros. eapply THEN_sound.
+  eapply APPLY_sound; eauto with typeclass_instances.
+  2: eapply MINIFY_sound.
+  intros. eapply exprUnify_sound; eauto with typeclass_instances.
+Qed.
+
+Definition even_odd_tac : rtac typ (expr typ func) :=
+  REPEAT 2000 (FIRST (APPLY E0_syn ::
+                      APPLY EO_syn ::
+                      APPLY OE_syn :: nil)).
+
+
+Definition build_n (n : nat) : expr typ func := Inj (inr n).
+
+Definition runRTac_empty_goal (tac : rtac typ (expr typ func))
+           (goal : expr typ func)  :=
+  (@runOnGoals _ _ _ _ tac)
+        nil nil 0 0 _ (@TopSubst _ _ nil nil)
+        (@GGoal typ (expr typ func) goal).
+
+Theorem even_odd_tac_sound
+: rtac_sound even_odd_tac.
+  eapply REPEAT_sound.
+  eapply FIRST_sound.
+  econstructor; [ eapply APPLY_sound; exact E0 | ].
+  constructor; [ eapply APPLY_sound; exact EO | ].
+  constructor; [ eapply APPLY_sound; exact OE | ].
+  constructor.
+Qed.
+
+
+(*Time Eval vm_compute in runRTac_empty_goal even_odd_tac (App Even_syn (build_n 1024)).*)
+
+Definition GoalD (us vs : env) (g : Goal typ (expr typ func)) : Prop :=
+  let (tus, us0) := split_env us in
+  let (tvs, vs0) := split_env vs in
+  match @goalD typ (expr typ func) _ _ _ tus tvs g with
+    | Some P => P us0 vs0
+    | None => False
+  end.
+
+Definition full_solved : @Result typ (expr typ func) (CTop nil nil) :=
+  Solved (TopSubst (expr typ func) nil nil).
+
+Theorem runGoal_sound
+: forall e,
+    runRTac_empty_goal even_odd_tac e = full_solved ->
+    GoalD nil nil (GGoal e).
+Proof.
+Admitted.
+
+Let Const (n : nat) : expr typ func := ExprCore.Inj (inr n).
+
+Definition pE0_syn : Lemma.lemma typ (expr typ func) (expr typ func) :=
+{| Lemma.vars := nil
+ ; Lemma.premises := nil
+ ; Lemma.concl := App Even_syn (Const 0)
+ |}.
+
+Definition pEO_syn (n : nat) : Lemma.lemma typ (expr typ func) (expr typ func) :=
+{| Lemma.vars := nil
+ ; Lemma.premises := App Odd_syn (Const n) :: nil
+ ; Lemma.concl := App Even_syn (Const (S n))
+ |}.
+
+Definition pOE_syn (n : nat) : Lemma.lemma typ (expr typ func) (expr typ func) :=
+{| Lemma.vars := nil
+ ; Lemma.premises := App Even_syn (Const n) :: nil
+ ; Lemma.concl := App Odd_syn (Const (S n))
+ |}.
+
+Definition even_odd_tac_nrec (fuel : nat) : rtac typ (expr typ func) :=
+  @REC _ _ fuel
+       (fun tac =>
+          AT_GOAL (fun _ _ e =>
+                     match e with
+                       | App (ExprCore.Inj (inl 3%positive))
+                             (ExprCore.Inj (inr 0)) =>
+                         APPLY pE0_syn
+                       | App (ExprCore.Inj (inl 3%positive))
+                             (ExprCore.Inj (inr (S n))) =>
+                         THEN (APPLY (pEO_syn n)) (runOnGoals tac)
+                       | App (ExprCore.Inj (inl 4%positive))
+                             (ExprCore.Inj (inr (S n))) =>
+                         THEN (APPLY (pOE_syn n)) (runOnGoals tac)
+                       | _ => FAIL
+                     end))
+       FAIL.
+
+Fixpoint even_odd_tac_mf (n : nat) : rtac typ (expr typ func) :=
+  match n with
+    | 0 => APPLY pE0_syn
+    | S n => THEN (FIRST (APPLY (pEO_syn n) :: APPLY (pOE_syn n) :: nil))
+                  (fun x => runOnGoals (even_odd_tac_mf n) x)
+  end.
+
+Theorem runGoal_sound_mf
+: forall n,
+    runRTac_empty_goal (even_odd_tac_mf n) (App Even_syn (Const n)) = full_solved ->
+    GoalD nil nil (GGoal (App Even_syn (Const n))).
+Proof.
+Admitted.
+
+Theorem runGoal_sound_nonrec
+: forall n,
+    runRTac_empty_goal (even_odd_tac_mf n) (App Even_syn (Const n)) = full_solved ->
+    GoalD nil nil (GGoal (App Even_syn (Const n))).
+Proof.
+Admitted.
+
+(*
+Time Eval vm_compute in let n := 2000 in runRTac_empty_goal (even_odd_tac_mf n) (App Even_syn (Const n)).
+
+Time Eval vm_compute in let n := 2000 in runRTac_empty_goal (even_odd_tac_nrec n) (App Even_syn (Const n)).
+*)
+
+Goal Even 512.
+  Time match goal with
+    | |- Even ?X =>
+      pose (GoalD nil nil (GGoal (App Even_syn (Const X)))) ;
+      apply (runGoal_sound_nonrec X); vm_compute; reflexivity
+  end.
+Time Qed.
